
Starting with the linear state space equation given by
\[
\ddot{z} =  - \frac{b}{m}\dot{z} - \frac{k}{m} z +  \frac{1}{m} F,
\]
and defining $x=(z, \dot{z})^\top$ and $u = F$ we get
\begin{align*}
  \dot{x}_1 = \dot{z} &= x_2 \\
  \dot{x}_2 = \ddot{z} &= - \frac{b}{m}\dot{z} - \frac{k}{m} z +  \frac{1}{m} F \\
  &= - \frac{b}{m} x_2 -  \frac{k}{m} x_1 + \frac{1}{m} u   \\
  y &= z = x_1.
\end{align*}
In matrix form
\begin{align*}
  \dot{x} &= \begin{pmatrix}
    \dot{x}_1 \\
    \dot{x}_2
  \end{pmatrix} =
  \begin{pmatrix}
    0 & 1 \\
    -\frac{k}{m} & - \frac{b}{m}
  \end{pmatrix}
  \begin{pmatrix}
    x_1 \\
    x_2
  \end{pmatrix}
  +
  \begin{pmatrix}
    0 \\
    \frac{1}{m}
  \end{pmatrix}
   u \\
   y &= \begin{pmatrix}
     1 & 0
   \end{pmatrix}
     \begin{pmatrix}
    x_1 \\
    x_2
  \end{pmatrix}
  +
  ( 0 ) u,
\end{align*}
or 
\begin{align*}
\dot{x} &= Ax + Bu \\
y &= Cx
\end{align*}
where
\begin{align*}
A&=\begin{pmatrix} 0 & 1 \\  -\frac{k}{m}  & -\frac{b}{m} \end{pmatrix} \\
B&=\begin{pmatrix} 0 \\ \frac{1}{m} \end{pmatrix} \\
C&=\begin{pmatrix} 1 & 0\end{pmatrix}.
\end{align*}
